\section*{Differentialrechnung}

\subsection*{Differenzenquotient}
$\Diff_{f,a}(x): U\setminus\{a\}\to\mathbb{R}: x\mapsto\frac{f(x)-f(a)}{x-a}$

\subsection*{Differenzierbarkeit/Ableitung}
$\displaystyle f'(x) := \lim_{x\to a}\Diff_{f,a}(x)$, sofern existiert

\textit{Stetigkeit:} diff.bar $\implies$ stetig

\subsection*{Rechenregeln}

\subsubsection*{Produktregel}
$(f \cdot g)'(a)=f'(a)\cdot g(a)+f(a)\cdot g'(a)$

\subsubsection*{Quotientenregel}
$\left(\frac{f}{g}\right)'(a)=\frac{f'(a)\cdot g(a) - f(a)\cdot g'(a)}{g(a)^2}$

\subsubsection*{Kettenregel}
$(g\circ f)'(a) = g'(f(a))\cdot f'(a)$

\subsection*{Umkehrfunktion}
$f$ diff.bar in $a$, $f'(a)\neq0$, $b=f(a)$ \\
$\implies (f^{-1})'(b) = \frac{1}{f'(a)}=\frac{1}{f'(f^{-1}(b))}$

\subsection*{Satz von de l'H\^opital}
$f,g$ auf $(a,b)$ diff.bar,

$\displaystyle \lim_{x\to c}f(x),g(x)=0 \lor
\lim_{x\to c}g(x)\in\{\infty,-\infty\}$

$\displaystyle \implies \lim_{x\to c}\frac{f(x)}{g(x)}=\lim_{x\to c}\frac{f'(x)}{g'(x)}$
